progs/message.v
@@ -1,0 +1,170 @@
+Require Import Clightdefs.
+
+Local Open Scope Z_scope.
+
+Definition _bufsize : ident := 15%positive.
+Definition _p : ident := 7%positive.
+Definition ___builtin_annot_intval : ident := 3%positive.
+Definition ___builtin_fabs : ident := 1%positive.
+Definition _serialize : ident := 14%positive.
+Definition _main : ident := 19%positive.
+Definition _intpair_serialize : ident := 9%positive.
+Definition _y : ident := 4%positive.
+Definition _q : ident := 17%positive.
+Definition _buf : ident := 8%positive.
+Definition _len : ident := 18%positive.
+Definition _struct_message : ident := 16%positive.
+Definition _deserialize : ident := 13%positive.
+Definition _struct_intpair : ident := 6%positive.
+Definition _intpair_message : ident := 12%positive.
+Definition _intpair_deserialize : ident := 11%positive.
+Definition _x : ident := 5%positive.
+Definition ___builtin_memcpy_aligned : ident := 2%positive.
+Definition _length : ident := 10%positive.
+
+Definition t_struct_intpair :=
+   (Tstruct _struct_intpair (Fcons _x tint (Fcons _y tint Fnil)) noattr).
+Definition t_struct_message :=
+   (Tstruct _struct_message
+     (Fcons _bufsize tint
+       (Fcons _serialize
+         (tptr (Tfunction (Tcons (tptr tvoid) (Tcons (tptr tuchar) Tnil))
+                 tint))
+         (Fcons _deserialize
+           (tptr (Tfunction
+                   (Tcons (tptr tvoid)
+                     (Tcons (tptr tuchar) (Tcons tint Tnil))) tvoid)) Fnil)))
+     noattr).
+
+Definition f_intpair_serialize := {|
+  fn_return := tint;
+  fn_params := ((_p, (tptr t_struct_intpair)) :: (_buf, (tptr tuchar)) ::
+                nil);
+  fn_vars := nil;
+  fn_temps := ((_x, tint) :: (_y, tint) :: nil);
+  fn_body :=
+(Ssequence
+  (Sset _x
+    (Efield (Ederef (Etempvar _p (tptr t_struct_intpair)) t_struct_intpair)
+      _x tint))
+  (Ssequence
+    (Sset _y
+      (Efield (Ederef (Etempvar _p (tptr t_struct_intpair)) t_struct_intpair)
+        _y tint))
+    (Ssequence
+      (Sassign
+        (Ederef
+          (Ebinop Oadd (Ecast (Etempvar _buf (tptr tuchar)) (tptr tint))
+            (Econst_int (Int.repr 0) tint) (tptr tint)) tint)
+        (Etempvar _x tint))
+      (Ssequence
+        (Sassign
+          (Ederef
+            (Ebinop Oadd (Ecast (Etempvar _buf (tptr tuchar)) (tptr tint))
+              (Econst_int (Int.repr 1) tint) (tptr tint)) tint)
+          (Etempvar _y tint))
+        (Sreturn (Some (Econst_int (Int.repr 8) tint)))))))
+|}.
+
+Definition f_intpair_deserialize := {|
+  fn_return := tvoid;
+  fn_params := ((_p, (tptr t_struct_intpair)) :: (_buf, (tptr tuchar)) ::
+                (_length, tint) :: nil);
+  fn_vars := nil;
+  fn_temps := ((_x, tint) :: (_y, tint) :: nil);
+  fn_body :=
+(Ssequence
+  (Sset _x
+    (Ederef
+      (Ebinop Oadd (Ecast (Etempvar _buf (tptr tuchar)) (tptr tint))
+        (Econst_int (Int.repr 0) tint) (tptr tint)) tint))
+  (Ssequence
+    (Sset _y
+      (Ederef
+        (Ebinop Oadd (Ecast (Etempvar _buf (tptr tuchar)) (tptr tint))
+          (Econst_int (Int.repr 1) tint) (tptr tint)) tint))
+    (Ssequence
+      (Sassign
+        (Efield
+          (Ederef (Etempvar _p (tptr t_struct_intpair)) t_struct_intpair) _x
+          tint) (Etempvar _x tint))
+      (Sassign
+        (Efield
+          (Ederef (Etempvar _p (tptr t_struct_intpair)) t_struct_intpair) _y
+          tint) (Etempvar _y tint)))))
+|}.
+
+Definition v_intpair_message := {|
+  gvar_info := t_struct_message;
+  gvar_init := (Init_int32 (Int.repr 8) ::
+                Init_addrof _intpair_serialize (Int.repr 0) ::
+                Init_addrof _intpair_deserialize (Int.repr 0) :: nil);
+  gvar_readonly := false;
+  gvar_volatile := false
+|}.
+
+Definition f_main := {|
+  fn_return := tint;
+  fn_params := nil;
+  fn_vars := ((_p, t_struct_intpair) :: (_q, t_struct_intpair) ::
+              (_buf, (tarray tuchar 8)) :: nil);
+  fn_temps := ((_len, tint) :: (_x, tint) :: (_y, tint) ::
+               (20%positive, tint) :: nil);
+  fn_body :=
+(Ssequence
+  (Sassign (Efield (Evar _p t_struct_intpair) _x tint)
+    (Econst_int (Int.repr 1) tint))
+  (Ssequence
+    (Sassign (Efield (Evar _p t_struct_intpair) _y tint)
+      (Econst_int (Int.repr 2) tint))
+    (Ssequence
+      (Ssequence
+        (Scall (Some 20%positive)
+          (Efield (Evar _intpair_message t_struct_message) _serialize
+            (tptr (Tfunction (Tcons (tptr tvoid) (Tcons (tptr tuchar) Tnil))
+                    tint)))
+          ((Eaddrof (Evar _p t_struct_intpair) (tptr t_struct_intpair)) ::
+           (Evar _buf (tarray tuchar 8)) :: nil))
+        (Sset _len (Etempvar 20%positive tint)))
+      (Ssequence
+        (Scall None
+          (Efield (Evar _intpair_message t_struct_message) _deserialize
+            (tptr (Tfunction
+                    (Tcons (tptr tvoid)
+                      (Tcons (tptr tuchar) (Tcons tint Tnil))) tvoid)))
+          ((Eaddrof (Evar _q t_struct_intpair) (tptr t_struct_intpair)) ::
+           (Evar _buf (tarray tuchar 8)) :: (Econst_int (Int.repr 8) tint) ::
+           nil))
+        (Ssequence
+          (Sset _x (Efield (Evar _q t_struct_intpair) _x tint))
+          (Ssequence
+            (Sset _y (Efield (Evar _q t_struct_intpair) _y tint))
+            (Sreturn (Some (Ebinop Oadd (Etempvar _x tint) (Etempvar _y tint)
+                             tint)))))))))
+|}.
+
+Definition prog : Clight.program := {|
+prog_defs :=
+((___builtin_fabs,
+   Gfun(External (EF_builtin ___builtin_fabs
+                   (mksignature (AST.Tfloat :: nil) (Some AST.Tfloat)))
+     (Tcons tdouble Tnil) tdouble)) ::
+ (___builtin_memcpy_aligned,
+   Gfun(External (EF_builtin ___builtin_memcpy_aligned
+                   (mksignature
+                     (AST.Tint :: AST.Tint :: AST.Tint :: AST.Tint :: nil)
+                     None))
+     (Tcons (tptr tvoid)
+       (Tcons (tptr tvoid) (Tcons tuint (Tcons tuint Tnil)))) tvoid)) ::
+ (___builtin_annot_intval,
+   Gfun(External (EF_builtin ___builtin_annot_intval
+                   (mksignature (AST.Tint :: AST.Tint :: nil)
+                     (Some AST.Tint)))
+     (Tcons (tptr tschar) (Tcons tint Tnil)) tint)) ::
+ (_intpair_serialize, Gfun(Internal f_intpair_serialize)) ::
+ (_intpair_deserialize, Gfun(Internal f_intpair_deserialize)) ::
+ (_intpair_message, Gvar v_intpair_message) ::
+ (_main, Gfun(Internal f_main)) :: nil);
+prog_main := _main
+|}.
+
