progs/verif_message.v
@@ -1,0 +1,139 @@
+Load loadpath.
+Require Import Coqlib msl.Coqlib2.
+Require Import veric.SeparationLogic.
+Require Import Ctypes.
+Require Import Clightdefs.
+Require veric.SequentialClight.
+Import SequentialClight.SeqC.CSL.
+Require Import progs.field_mapsto.
+Require Import progs.client_lemmas.
+Require Import progs.assert_lemmas.
+Require Import progs.forward.
+Require Import progs.malloc_lemmas.
+Require Import progs.message.
+
+Local Open Scope logic.
+
+(* f : message_format t
+    f sh buf n data  := the [data] is formatted into a message of length [n]
+          stored starting at address [buf] with share [sh] *)
+Definition message_format (t: type) : Type :=
+   forall (sh: share) (buf: val) (length:  Z) (data: reptype t), mpred.
+
+Definition intpair_message: message_format t_struct_intpair :=
+  fun sh buf n data => 
+   !!(n= sizeof t_struct_intpair) && typed_mapsto t_struct_intpair sh buf data.
+
+Definition serialize_spec {t: type} (format: message_format t) :=
+  WITH data: reptype t, p: val, buf: val, sh: share, sh': share
+  PRE [ _p OF (tptr t), _buf OF (tptr tuchar) ] 
+          PROP (writable_share sh')
+          LOCAL (`(eq p) (eval_id _p); `(eq buf) (eval_id _buf))
+          SEP (`(typed_mapsto t sh p data); 
+                 `(memory_block sh' (Int.repr (sizeof t)) buf))
+  POST [ tint ] 
+         `(typed_mapsto t sh p data) 
+           * `(format sh' buf) (`Int.unsigned (`force_int retval)) `data.
+
+Definition deserialize_spec {t: type} (format: message_format t) :=
+  WITH data: reptype t, p: val, buf: val, sh: share, sh': share
+  PRE [ _p OF (tptr t), _buf OF (tptr tuchar), _length OF tint ] 
+          PROP (writable_share sh)
+          LOCAL (`(eq p) (eval_id _p); `(eq buf) (eval_id _buf))
+          SEP (`(format sh' buf) (`Int.unsigned (`force_int (eval_id _length))) `data;
+                 `(memory_block sh' (Int.repr (sizeof t)) p))
+  POST [ tint ]
+            `(format sh' buf) (`Int.unsigned (`force_int (eval_id _length))) `data *
+            `(typed_mapsto t sh p data).
+
+Definition intpair_serialize_spec :=
+ DECLARE _intpair_serialize (serialize_spec intpair_message).
+
+Definition intpair_deserialize_spec :=
+ DECLARE _intpair_deserialize (deserialize_spec intpair_message).
+
+Definition main_spec :=
+ DECLARE _main
+  WITH u : unit
+  PRE  [] main_pre prog u
+  POST [ tint ] main_post prog u.
+
+Definition Vprog : varspecs := (_intpair_message, t_struct_message)::nil.
+
+Definition func_at (spec: funspec) (v: val) : mpred := 
+  match v with Vptr b z => veric.seplog.func_at spec (b, Int.unsigned z)
+   | _ => FF
+  end.
+
+Definition message {t: type} (format: message_format t) (sh: share) (m: val) : mpred :=
+  EX fg: val*val,
+          func_at (serialize_spec format) (fst fg) &&
+          func_at (deserialize_spec format) (snd fg) &&
+       typed_mapsto t_struct_message sh m (Int.repr (sizeof t), (fst fg, snd fg)).
+
+Definition Gprog : funspecs := 
+    intpair_serialize_spec :: intpair_deserialize_spec :: main_spec::nil.
+
+Definition Gtot := do_builtins (prog_defs prog) ++ Gprog.
+
+Lemma body_intpair_serialize: semax_body Vprog Gtot f_intpair_serialize intpair_serialize_spec.
+Proof.
+unfold intpair_serialize_spec.
+unfold serialize_spec.
+start_function.
+name p0 _p.
+name buf0 _buf.
+name x _x.
+name y _y.
+rewrite memory_block_typed.
+do 2 simpl_typed_mapsto.
+destruct data as (x1,y1); simpl in *.
+apply semax_pre_PQR with
+ (PROP  (isptr buf)
+   LOCAL  (`(eq p) (eval_id _p); `(eq buf) (eval_id _buf))
+   SEP 
+   (`(field_mapsto sh t_struct_intpair _x) (eval_id _p) `(Vint x1);
+    `(field_mapsto sh t_struct_intpair _y) (eval_id _p) `(Vint y1);
+   `(mapsto_ sh' tint) (`(add_ptr_int tint) (`(eval_cast (tptr tuchar) (tptr tint)) (eval_id _buf)) `0);
+   `(mapsto_ sh' tint) (`(add_ptr_int tint) (`(eval_cast (tptr tuchar) (tptr tint)) (eval_id _buf)) `1))).
+go_lower; subst;  rewrite (field_mapsto__isptr). normalize. 
+ cancel.
+apply sepcon_derives; apply derives_refl''; 
+ eapply mapsto_field_mapsto_; unfold field_offset; try (simpl; reflexivity);
+ apply add_ptr_int_offset;
+ simpl; compute; intuition congruence.
+forward. (* x = p->x; *)
+forward. (* y = p->y; *)
+forward. (*  ((int * )buf)[0]=x; *)
+go_lower. subst. apply andp_right; auto. apply prop_right; intuition.
+forward. (*  ((int * )buf)[1]=y; *)
+go_lower. subst. apply andp_right; auto. apply prop_right; intuition.
+forward. (* return 8; *)
+go_lower. subst. apply andp_right; try apply prop_right; auto.
+unfold intpair_message.
+normalize.
+cancel.
+simpl_typed_mapsto.
+simpl.
+rewrite sepcon_comm.
+apply sepcon_derives; apply derives_refl';
+ eapply mapsto_field_mapsto; unfold field_offset; try (simpl; reflexivity);
+destruct buf0; inv H0; reflexivity.
+Qed.
+
+
+
+
+
+
+
+
+
+
+
+
+
+
+
+
+
